specs/Spec.LZ77.fst
@@ -1,78 +1,414 @@
 module Spec.LZ77
 
+module B = LowStar.Buffer
 module Cast = FStar.Int.Cast
+module CB = LowStar.ConstBuffer
+module CFlags = Yazi.CFlags
+module HS = FStar.HyperStack
+module I32 = FStar.Int32
+module LB = Lib.Buffer
+module Math = FStar.Math.Lemmas
+module U8 = FStar.UInt8
 module U16 = FStar.UInt16
 module U32 = FStar.UInt32
-module UInt = FStar.UInt
 
 open FStar.Mul
 open Lib.UInt
+open Lib.Seq
+open Yazi.LZ77.Types
 
-unfold let (^) #n = UInt.logxor #n
-unfold let (&@) #n = UInt.logand #n
-unfold let (<<) #n = UInt.shift_left #n
+let min_match = 4
+let max_match = 258
+let min_lookhead = max_match + min_match + 1
 
-#set-options "--fuel 4 --ifuel 4"
-let triple_shift_zero
-  (#n: hash_bits)
-  (shift: hash_shift n)
-  (mask: hash_mask n)
-  (a: U8.t): Lemma
-  (ensures (((U16.v (Cast.uint8_to_uint16 a)) << (3 * shift)) &@ mask) == 0) =
-  assert(3 * shift >= n);
-  hash_mask_ones n;
-  let a' = (U16.v (Cast.uint8_to_uint16 a)) << (3 * shift) in
-  assert(Seq.equal (UInt.to_vec (a' &@ mask)) (UInt.to_vec (UInt.zero 16)))
+unfold let is_hash_bits (b: nat) = b >= 8 /\ b <= 16
+type hash_bits = b: nat{is_hash_bits b}
 
-#set-options "--fuel 0 --ifuel 0"
-let roll_hash_eq bits m s a b c d h =
+unfold let is_hash_mask (bits: hash_bits) (m: nat) = m == (pow2 bits) - 1
+type hash_mask (bits: hash_bits) = m: nat{is_hash_mask bits m}
+
+unfold let is_hash_size (bits: hash_bits) (s: nat) = s == pow2 bits
+type hash_size (bits: hash_bits) = s: nat{is_hash_size bits s}
+
+unfold let is_window_bits (b: nat) = b >= 8 /\ b <= 15
+type window_bits = b: nat{is_window_bits b}
+
+unfold let is_window_mask (b: window_bits) (m: nat) = m == (pow2 b) - 1
+type window_mask (bits: window_bits) = m: nat{is_window_mask bits m}
+
+unfold let is_window_size (b: window_bits) (s: nat) = s == pow2 b
+type window_size (bits: window_bits) = s: nat{is_window_size bits s}
+
+let window_size_upper_bound (b: window_bits) (w_size: window_size b): Lemma
+  (ensures w_size <= 32768) = assert_norm(w_size == pow2 b)
+
+let context_valid (h: HS.mem) (ctx: lz77_context_p) =
   let open U16 in
-  let m' = v m in
-  let s' = v s in
-  let a' = Cast.uint8_to_uint16 a in
-  let b' = Cast.uint8_to_uint16 b in
-  let c' = Cast.uint8_to_uint16 c in
-  let d' = Cast.uint8_to_uint16 d in
-  let a'' = v a' in
-  let b'' = v b' in
-  let c'' = v c' in
-  let d'' = v d' in
-  let h' = ((h <<^ (Cast.uint16_to_uint32 s)) ^^ d') &^ m in
-  UInt.shift_left_logand_lemma (((a'' << (2 * s')) ^ (b'' << s')) ^ c'') m' s';
-  UInt.shift_left_logxor_lemma ((a'' << (2 * s')) ^ (b'' << s')) c'' s';
-  UInt.shift_left_logxor_lemma (a'' << (2 * s')) (b'' << s') s';
-  logxor_logand_distr
-    ((((a'' << (3 * s')) ^ (b'' << (2 * s'))) ^ (c'' << s')) &@ (m' << s'))
-    d''
-    m';
-  UInt.logand_associative
-    (((a'' << (3 * s')) ^ (b'' << (2 * s'))) ^ (c'' << s'))
-    (m' << s')
-    m';
-  UInt.logand_commutative (m' << s') m';
-  UInt.logand_associative
-    (((a'' << (3 * s')) ^ (b'' << (2 * s'))) ^ (c'' << s'))
-    m'
-    (m' << s');
-  logxor_logand_distr
-    ((a'' << (3 * s')) ^ (b'' << (2 * s')))
-    (c'' << s')
-    m';
-  logxor_logand_distr (a'' << (3 * s')) (b'' << (2 * s')) m';
-  triple_shift_zero #bits s' m' a;
-  UInt.logxor_commutative 0 ((b'' << (2 * s')) &@ m');
-  UInt.logxor_lemma_1 ((b'' << (2 * s')) &@ m');
-  logxor_logand_distr (b'' << (2 * s')) (c'' << s') m';
-  shift_left_append b'' s' s';
-  UInt.shift_left_logxor_lemma (b'' << s') c'' s';
-  UInt.logand_associative (((b'' << s') ^ c'') << s') m' (m' << s');
-  UInt.logand_associative (((b'' << s') ^ c'') << s') (m' << s') m';
-  UInt.shift_left_logand_lemma ((b'' << s') ^ c'') m' s';
-  logxor_logand_distr ((((b'' << s') ^ c'') &@ m') << s') d'' m';
-  assert(forall (i: nat{i < 16}).
-    UInt.nth (((((b'' << s') ^ c'') &@ m') << s') &@ m') i ==
-    UInt.nth ((((b'' << s') ^ c'') << s') &@ m') i);
-  UInt.to_vec_lemma_2
-    (((((b'' << s') ^ c'') &@ m') << s') &@ m')
-    ((((b'' << s') ^ c'') << s') &@ m');
-  logxor_logand_distr (((b'' << s') ^ c'') << s') d'' m'
+  CB.length ctx == 1 /\
+  (let c = B.get h (CB.as_mbuf ctx) 0 in
+  is_window_bits (v c.w_bits) /\
+  is_window_mask (v c.w_bits) (v c.w_mask) /\
+  is_window_size (v c.w_bits) (U32.v c.w_size) /\
+  U32.v c.window_size == (U32.v c.w_size) * 2 /\
+  B.length c.window == U32.v c.window_size /\
+  B.length c.prev == U32.v c.w_size /\
+  is_hash_bits (v c.h_bits) /\
+  is_hash_size (v c.h_bits) (U32.v c.h_size) /\
+  is_hash_mask (v c.h_bits) (v c.h_mask) /\
+  U32.v c.window_size - min_match + 1 > U32.v c.w_size /\
+  B.length c.head == U32.v c.h_size /\
+  CB.live h ctx /\ B.live h c.prev /\ B.live h c.window /\ B.live h c.head /\ B.live h c.prev /\
+  B.disjoint c.window c.prev /\ B.disjoint c.window c.head /\ B.disjoint c.prev c.head /\
+  B.frameOf c.window == B.frameOf c.prev /\ B.frameOf c.prev == B.frameOf c.head /\
+  B.frameOf (CB.as_mbuf ctx) <> B.frameOf c.prev /\
+  HS.disjoint (B.frameOf (CB.as_mbuf ctx)) (B.frameOf c.prev))
+
+noextract private type valid_context_p (h: HS.mem) =
+  ctx: lz77_context_p{context_valid h ctx}
+
+let window_index_upper_bound (h: HS.mem) (ctx: valid_context_p h) (i: nat): Lemma
+  (requires i < (U32.v (B.get h (CB.as_mbuf ctx) 0).window_size))
+  (ensures i < pow2 16) =
+  let ctx' = B.get h (CB.as_mbuf ctx) 0 in
+  calc (<) {
+    i;
+    <{}
+    U32.v ctx'.window_size;
+    =={}
+    2 * pow2 (U16.v ctx'.w_bits);
+    <={Math.Lemmas.pow2_le_compat 15 (U16.v ctx'.w_bits)}
+    2 * pow2 15;
+    =={Math.Lemmas.pow2_double_mult 15}
+    pow2 16;
+  }
+
+#set-options "--z3rlimit 120 --fuel 0 --ifuel 0"
+let window_mask_aux
+  (w_bits: window_bits)
+  (w_size: window_size w_bits)
+  (w_mask: window_mask w_bits)
+  (i: UInt.uint_t 32): Lemma
+  (requires i < 2 * w_size)
+  (ensures
+    (i < w_size ==> UInt.logand i (UInt.to_uint_t 32 w_mask) == i) /\
+    (i >= w_size ==> UInt.logand i (UInt.to_uint_t 32 w_mask) == i - w_size)) =
+  UInt.logand_mask i w_bits;
+
+  if i < w_size then
+    ()
+  else
+    calc (==) {
+      UInt.logand i (UInt.to_uint_t 32 w_mask);
+      =={}
+      i % (pow2 w_bits);
+      =={Math.Lemmas.lemma_mod_sub i w_size 1}
+      (i - w_size) % w_size;
+      =={Math.Lemmas.small_mod (i - w_size) w_size}
+      i - w_size;
+    }
+
+assume val hash: (bits: hash_bits) -> U8.t -> U8.t -> U8.t -> U8.t -> Tot (res: U32.t{
+  U32.v res < pow2 bits
+})
+
+let hash_neq (bits: hash_bits) (a b c d: U8.t): Lemma
+  (ensures forall (a' b' c' d': U8.t). hash bits a b c d <> hash bits a' b' c' d' ==>
+    a <> a' \/ b <> b' \/ c <> c' \/ d <> d') = ()
+
+let hash_loc_buffer (h: HS.mem) (ctx: valid_context_p h) =
+  let ctx' = B.get h (CB.as_mbuf ctx) 0 in
+  (B.loc_buffer ctx'.head) `B.loc_union`
+  (if CFlags.fastest then B.loc_none else B.loc_buffer ctx'.prev)
+
+type hash_range (h: HS.mem) (ctx: valid_context_p h) =
+  hr: U32.t {U32.v hr <= U32.v (B.get h (CB.as_mbuf ctx) 0).window_size - min_match + 1}
+
+type slided_flag (#h: HS.mem) (#ctx: valid_context_p h) (hr: hash_range h ctx) = b: bool{
+  b == true ==> U32.v hr >= U32.v (B.get h (CB.as_mbuf ctx) 0).w_size
+}
+
+let slided_value
+  (#h: HS.mem)
+  (ctx: valid_context_p h)
+  (h_range: hash_range h ctx)
+  (slided: slided_flag h_range) =
+  let open U32 in
+  let ctx' = B.get h (CB.as_mbuf ctx) 0 in
+  let h_range' = if slided then h_range -^ ctx'.w_size else h_range in
+  let window' = if slided then 
+    B.as_seq h (B.gsub ctx'.window ctx'.w_size ctx'.w_size)
+  else
+    B.as_seq h ctx'.window
+  in
+  (U32.v h_range', window')
+
+unfold let sub_head_valid
+  (h: HS.mem)
+  (ctx: valid_context_p h)
+  (h_range: hash_range h ctx)
+  (range: (i: nat) -> (p:Type0{p ==> i < U32.v (B.get h (CB.as_mbuf ctx) 0).h_size}))
+  (slided: slided_flag h_range) =
+  let open U32 in
+  let ctx' = B.get h (CB.as_mbuf ctx) 0 in
+  let head' = B.as_seq h ctx'.head in
+  let (h_range', window') = slided_value ctx h_range slided in
+  (forall (i: nat{range i /\ U16.v head'.[i] <> 0}).
+    let h_bits = U16.v ctx'.h_bits in
+    let head = U16.v head'.[i] in
+    head < h_range' /\
+    i == v (hash
+      h_bits
+      window'.[head]
+      window'.[head + 1]
+      window'.[head + 2]
+      window'.[head + 3]))
+
+unfold let head_valid
+  (h: HS.mem)
+  (ctx: valid_context_p h)
+  (h_range: hash_range h ctx)
+  (slided: slided_flag h_range) =
+  sub_head_valid h ctx h_range (fun j -> j < U32.v (B.get h (CB.as_mbuf ctx) 0).h_size) slided
+
+let sub_prev_valid
+  (h: HS.mem)
+  (ctx: valid_context_p h)
+  (h_range: hash_range h ctx)
+  (range: (i: nat) -> (p:Type0{p ==> i < U32.v (B.get h (CB.as_mbuf ctx) 0).w_size}))
+  (slided: slided_flag h_range) =
+  let open U32 in let open Lib.Seq in
+  let ctx' = B.get h (CB.as_mbuf ctx) 0 in
+  let prev' = B.as_seq h ctx'.prev in
+  let (h_range', w) = slided_value ctx h_range slided in
+  let hash = hash (U16.v ctx'.h_bits) in
+  (h_range' > 0 ==> (forall (i: nat{range i}).
+    let b = U16.v prev'.[i] in
+    let b' = i + v ctx'.w_size in
+    b < h_range' /\
+    (b <> 0 ==>
+      ((b' < h_range' ==>
+        (b < i + v ctx'.w_size /\
+        hash w.[b] w.[b + 1] w.[b + 2] w.[b + 3] ==
+        hash w.[b'] w.[b' + 1] w.[b' + 2] w.[b' + 3]))) /\
+      (h_range' <= b' /\ i < h_range' ==>
+        (b < i /\
+        hash w.[b] w.[b + 1] w.[b + 2] w.[b + 3] ==
+        hash w.[i] w.[i + 1] w.[i + 2] w.[i + 3])))))
+
+let prev_valid
+  (h: HS.mem)
+  (ctx: valid_context_p h)
+  (h_range: hash_range h ctx)
+  (slided: slided_flag h_range) =
+  sub_prev_valid h ctx h_range (fun j ->
+    let open U32 in
+    let ctx' = B.get h (CB.as_mbuf ctx) 0 in
+    if v h_range >= v ctx'.w_size then
+      j < U32.v (B.get h (CB.as_mbuf ctx) 0).w_size
+    else
+      j < U32.v h_range)
+    slided
+
+unfold let hash_chain_valid
+  (h: HS.mem)
+  (ctx: valid_context_p h)
+  (h_range: hash_range h ctx)
+  (slided: slided_flag h_range) =
+  (CFlags.fastest == false ==> prev_valid h ctx h_range slided) /\
+  head_valid h ctx h_range slided
+
+type lz77_state = s:Seq.seq U32.t{Seq.length s == 7}
+
+unfold let match_length (s: lz77_state) = U32.v s.[0]
+unfold let match_start (s: lz77_state) = U32.v s.[1]
+unfold let prev_match (s: lz77_state) = U32.v s.[2]
+unfold let prev_length (s: lz77_state) = U32.v s.[3]
+unfold let strstart (s: lz77_state) = U32.v s.[4]
+unfold let lookahead (s: lz77_state) = U32.v s.[5]
+unfold let insert (s: lz77_state) = U32.v s.[6]
+unfold let window_end (s: lz77_state) = strstart s + lookahead s
+unfold let max_hash_end (s: lz77_state) = window_end s - min_match + 1
+
+unfold let match_length_unchange (s0 s1: lz77_state) = match_length s0 == match_length s1
+unfold let match_start_unchange (s0 s1: lz77_state) = match_start s0 == match_start s1
+unfold let prev_match_unchange (s0 s1: lz77_state) = prev_match s0 == prev_match s1
+unfold let prev_length_unchange (s0 s1: lz77_state) = prev_length s0 == prev_length s1
+unfold let strstart_unchange (s0 s1: lz77_state) = strstart s0 == strstart s1
+unfold let lookahead_unchange (s0 s1: lz77_state) = lookahead s0 == lookahead s1
+unfold let insert_unchange (s0 s1: lz77_state) = insert s0 == insert s1
+
+// This condition should hold in all acases for all LZ77 states.
+let state_valid (h: HS.mem) (ctx: lz77_context_p) (s: lz77_state_t) =
+  context_valid h ctx /\ B.live h s /\
+  B.disjoint (CB.as_mbuf ctx) s /\
+  (let ctx' = B.get h (CB.as_mbuf ctx) 0 in
+  let s' = B.as_seq h s in
+  HS.disjoint (B.frameOf s) (B.frameOf ctx'.head) /\
+  
+  strstart s' + lookahead s' <= 2 * U32.v ctx'.w_size /\
+  insert s' <= strstart s' /\
+  match_length s' <= min_match /\
+  prev_length s' <= min_match /\
+  match_start s' <= 2 * U32.v ctx'.w_size - min_match /\
+  prev_match s' <= 2 * U32.v ctx'.w_size - min_match)
+
+let do_init_input_hash_pre
+  (h: HS.mem)
+  (ctx: lz77_context_p)
+  (state: lz77_state_t)
+  (i lk: U32.t)
+  (ins: UInt.uint_t 32) =
+    let open U32 in
+    let state' = B.as_seq h state in
+    state_valid h ctx state /\
+    strstart state' - insert state' == v i /\
+    v i < strstart state' /\
+    lookahead state' + insert state' >= min_match /\
+    hash_chain_valid h ctx i false /\
+    v lk == lookahead state' /\
+    ins == insert state'
+
+let do_init_input_hash_post (h0 h1: HS.mem) (ctx: lz77_context_p) (state: lz77_state_t) =
+  let s0 = B.as_seq h0 state in
+  let s1 = B.as_seq h1 state in
+  let e0 = max_hash_end s1 in
+  let e1 = strstart s1 in
+  state_valid h0 ctx state /\
+  B.modifies ((B.loc_buffer state) `B.loc_union` hash_loc_buffer h0 ctx) h0 h1 /\
+  LB.unchange_except h0 h1 state 6 /\
+  state_valid h1 ctx state /\
+  (e0 >= 0 /\ e1 >= 0 ==>
+    (e0 < e1 ==> hash_chain_valid h1 ctx (U32.uint_to_t e0) false) /\
+    (e1 <= e0 ==> hash_chain_valid h1 ctx (U32.uint_to_t e1) false))
+
+let init_input_hash_pre (h: HS.mem) (ctx: lz77_context_p) (state: lz77_state_t) =
+  let state' = B.as_seq h state in
+  B.live h state /\
+  (lookahead state' + insert state' >= min_match ==>
+    state_valid h ctx state /\
+    hash_chain_valid h ctx (U32.uint_to_t (strstart state' - insert state')) false)
+
+let init_input_hash_post (h0 h1: HS.mem) (ctx: lz77_context_p) (state: lz77_state_t) =
+  let s0 = B.as_seq h0 state in
+  (lookahead s0 + insert s0 >= min_match ==> do_init_input_hash_post h0 h1 ctx state) /\
+  (lookahead s0 + insert s0 < min_match ==> B.modifies B.loc_none h0 h1)
+
+let do_init_dict_hash_pre
+  (h: HS.mem)
+  (ctx: lz77_context_p)
+  (state: lz77_state_t)
+  (i: U32.t)
+  (h_end: UInt.uint_t 32) =
+    let open U32 in
+    let state' = B.as_seq h state in
+    state_valid h ctx state /\
+    lookahead state' >= min_match /\
+    strstart state' <= v i /\ v i < max_hash_end state' /\
+    hash_chain_valid h ctx i false /\
+    h_end == max_hash_end state'
+
+let do_init_dict_hash_post (h0 h1: HS.mem) (ctx: lz77_context_p) (state: lz77_state_t) =
+  let state' = B.as_seq h0 state in
+  state_valid h0 ctx state /\
+  lookahead state' >= min_match /\
+  B.modifies (hash_loc_buffer h0 ctx) h0 h1 /\
+  state_valid h1 ctx state /\
+  hash_chain_valid h1 ctx (U32.uint_to_t (max_hash_end state')) false
+  
+unfold let init_dict_hash_pre (h: HS.mem) (ctx: lz77_context_p) (state: lz77_state_t) =
+  let state' = B.as_seq h state in
+  B.live h state /\
+  state_valid h ctx state /\
+  lookahead state' >= min_match /\
+  hash_chain_valid h ctx (U32.uint_to_t (strstart state')) false
+
+unfold let init_dict_hash_post (h0 h1: HS.mem) (ctx: lz77_context_p) (state: lz77_state_t) =
+  let state' = B.as_seq h1 state in
+  init_dict_hash_pre h0 ctx state /\
+  B.modifies (hash_loc_buffer h0 ctx) h0 h1 /\
+  state_valid h1 ctx state /\
+  hash_chain_valid h1 ctx (U32.uint_to_t (max_hash_end state')) false
+
+// TODO: verify block_start's lower bound
+unfold let slide_window_pre
+  (h: HS.mem)
+  (ctx: lz77_context_p)
+  (state: lz77_state_t)
+  (block_start: B.pointer I32.t) =
+  let open U32 in
+  let state' = B.as_seq h state in
+  state_valid h ctx state /\
+  (let ctx' = B.get h (CB.as_mbuf ctx) 0 in
+  B.live h block_start /\
+  B.disjoint (CB.as_mbuf ctx) block_start /\ B.disjoint state block_start /\
+  HS.disjoint (B.frameOf block_start) (B.frameOf ctx'.head) /\
+    
+  match_start state' >= v ctx'.w_size /\
+  strstart state' >= v ctx'.w_size /\
+  insert state' <= strstart state' - v ctx'.w_size /\
+  strstart state' - insert state' < v ctx'.window_size - min_match + 1 /\
+  I32.v (B.get h block_start 0) >= -8454144)
+
+private unfold let slide_window_buf_post'
+  (h0 h1: HS.mem)
+  (ctx: lz77_context_p)
+  (state: lz77_state_t)
+  (block_start: B.pointer I32.t)
+  (len: nat) =
+  state_valid h0 ctx state /\
+  (let ctx' = B.get h0 (CB.as_mbuf ctx) 0 in
+  let s0 = B.as_seq h0 state in
+  let s1 = B.as_seq h1 state in
+  let w0 = B.as_seq h0 ctx'.window in
+  let w1 = B.as_seq h1 ctx'.window in
+  let w_size' = U32.v ctx'.w_size in
+  match_length_unchange s0 s1 /\
+  prev_match_unchange s0 s1 /\ prev_length_unchange s0 s1 /\
+  lookahead_unchange s0 s1 /\ insert_unchange s0 s1 /\
+  
+  strstart s0 - U32.v ctx'.w_size == strstart s1 /\
+  match_start s0 - U32.v ctx'.w_size == match_start s1 /\
+
+  len <= U32.v ctx'.w_size /\
+  I32.v (B.get h0 block_start 0) - U32.v ctx'.w_size == I32.v (B.get h1 block_start 0) /\
+  Seq.slice w0 w_size' (w_size' + len) == Seq.slice w1 0 len)
+
+let slide_window_buf_post
+  (h0 h1: HS.mem)
+  (ctx: lz77_context_p)
+  (state: lz77_state_t)
+  (block_start: B.pointer I32.t)
+  (len: nat) =
+  slide_window_buf_post' h0 h1 ctx state block_start len /\
+  B.modifies (
+    B.loc_buffer block_start `B.loc_union`
+    B.loc_buffer state `B.loc_union`
+    B.loc_buffer (B.get h0 (CB.as_mbuf ctx) 0).window) h0 h1 /\
+  state_valid h1 ctx state
+
+unfold let slide_window_post
+  (h0: HS.mem) (more: U32.t) (h1: HS.mem)
+  (ctx: lz77_context_p{context_valid h0 ctx})
+  (state: lz77_state_t)
+  (block_start: B.pointer I32.t) =
+  let open U32 in
+  let ctx' = B.get h0 (CB.as_mbuf ctx) 0 in
+  let s0 = B.as_seq h0 state in
+  let s1 = B.as_seq h1 state in
+  slide_window_pre h0 ctx state block_start /\
+  
+  (strstart s0 < v ctx'.w_size ==> 
+    v more == 2 * v ctx'.w_size - lookahead s0 - strstart s0 /\
+    B.modifies B.loc_none h0 h1) /\
+  (strstart s0 >= U32.v ctx'.w_size ==>
+    v more == 2 * v ctx'.w_size - lookahead s0 - strstart s0 + v ctx'.w_size /\
+    B.modifies (
+      B.loc_buffer block_start `B.loc_union`
+      B.loc_buffer state `B.loc_union`
+      B.loc_buffer ctx'.window `B.loc_union`
+      hash_loc_buffer h0 ctx) h0 h1 /\
+    (let len = strstart s1 + lookahead s1 in
+    slide_window_buf_post' h0 h1 ctx state block_start len /\
+    len <= v ctx'.w_size /\
+    hash_chain_valid h1 ctx (uint_to_t (strstart s1 - insert s1)) false /\
+    state_valid h1 ctx state))
